Added completeness and monotonicity instances for AFI ty and tm relations

src/Language/PlutusIR/Semantics/Static/Theorems/ContextInvariance/AFI/DecOpt.v
@@ -29,13 +29,58 @@ Proof. (* derive_mon. Qed. *) idtac "Admitted: DecOptappears_free_in_ty_mon". Ad
 
 
 
-
-
-
 MetaCoq Run (deriveCTProxy appears_free_in_tm).
 
 Lemma appears_free_in_tm_proxy_sound : appears_free_in_tm_proxy_sound_type.
 Proof. deriveCTProxy_sound core. Qed.
+
+(* NOTE: I did not want to add the derivation for this proof type to CTProxy, since it
+   is more complex than for the sound proof type, and for now it only seems to be necessary 
+   for the proxy derived for the AFI relations.
+
+   Another thing to note is that simply using auto also 'seems' to work, however, it simply
+   applies the recursive functions without unfolding some underlying arguments. This is necessary
+   since fixpoint need a decreasing argument, thus some of that unfolding has to be done manually
+*)
+Fixpoint appears_free_in_tm_tm_proxy_complete x x' (H: appears_free_in_tm x x') {struct H} : 
+  appears_free_in_tm_proxy (appears_free_in_tm_tag x x')
+with appears_free_in_tm_bindings_nonrec_proxy_complete x x' (H : appears_free_in_tm__bindings_nonrec x x') {struct H} :
+  appears_free_in_tm_proxy (appears_free_in_tm__bindings_nonrec_tag x x')
+with appears_free_in_tm_bindings_rec_proxy_complete x x' (H: appears_free_in_tm__bindings_rec x x') {struct H} :
+  appears_free_in_tm_proxy (appears_free_in_tm__bindings_rec_tag x x')
+with appears_free_in_tm_binding_proxy_complete x x' (H: appears_free_in_tm__binding x x') {struct H} :
+  appears_free_in_tm_proxy (appears_free_in_tm__binding_tag x x').
+Proof with auto.
+  - inversion H; subst.
+    1: constructor; auto.
+    1: apply AFIT_LetNonRec_proxy; auto.
+    1: apply AFIT_LetRec_proxy; auto.
+    5: apply AFIT_Apply2_proxy; auto.
+    all: constructor; auto.
+  - inversion H; subst.
+    + constructor; auto.
+    + apply AFIT_ConsB2_NonRec_proxy; auto.
+  - inversion H; subst.
+    + constructor; auto.
+    + apply AFIT_ConsB2_Rec_proxy; auto.
+  - inversion H; subst. constructor. auto.
+Qed.
+
+Lemma appears_free_in_tm_proxy_complete : forall tag,
+    match tag with
+    | appears_free_in_tm__binding_tag x x0 => appears_free_in_tm__binding x x0
+    | appears_free_in_tm__bindings_rec_tag x x0 => appears_free_in_tm__bindings_rec x x0
+    | appears_free_in_tm__bindings_nonrec_tag x x0 => appears_free_in_tm__bindings_nonrec x x0
+    | appears_free_in_tm_tag x x0 => appears_free_in_tm x x0
+    end -> 
+    appears_free_in_tm_proxy tag.
+Proof with auto.
+  intros tag H. destruct tag.
+  - apply appears_free_in_tm_binding_proxy_complete...
+  - apply appears_free_in_tm_bindings_rec_proxy_complete...
+  - apply appears_free_in_tm_bindings_nonrec_proxy_complete...
+  - apply appears_free_in_tm_tm_proxy_complete...
+Qed.
 
 
 
@@ -43,6 +88,12 @@ QCDerive DecOpt for (appears_free_in_tm_proxy tag).
 
 Instance DecOptappears_free_in_tm_proxy_sound tag : DecOptSoundPos (appears_free_in_tm_proxy tag).
 Proof. (* derive_sound. Qed. *) idtac "Admitted: DecOptappears_free_in_tm_proxy_sound". Admitted.
+
+Instance DecOptappears_free_in_tm_proxy_complete tag : DecOptCompletePos (appears_free_in_tm_proxy tag).
+Proof. (* derive_complete. Qed. *) idtac "Admitted: DecOptappears_free_in_tm_proxy_complete". Admitted.
+
+Instance DecOptappears_free_in_tm_proxy_mon tag: DecOptSizeMonotonic (appears_free_in_tm_proxy tag).
+Proof. (* derive_mon. Qed. *) idtac "Admitted: DecOptappears_free_in_tm_proxy_mon". Admitted.
 
 
 (* appears_free_in_tm *)
@@ -52,6 +103,12 @@ Instance DecOptappears_free_in_tm name tm : DecOpt (appears_free_in_tm name tm) 
 
 Instance DecOptappears_free_in_tm_sound name tm : DecOptSoundPos (appears_free_in_tm name tm).
 Proof. derive__sound (appears_free_in_tm_proxy_sound (appears_free_in_tm_tag name tm)). Qed.
+
+Instance DecOptappears_free_in_tm_complete name tm : DecOptCompletePos (appears_free_in_tm name tm).
+Proof. derive__complete (appears_free_in_tm_proxy_complete). Qed.
+
+Instance DecOptappears_free_in_tm_mon name tm: DecOptSizeMonotonic (appears_free_in_tm name tm).
+Proof. apply DecOptappears_free_in_tm_proxy_mon. Qed.
 
 
 
@@ -63,6 +120,12 @@ Instance DecOptappears_free_in_tm__bindings_nonrec bs tm : DecOpt (appears_free_
 Instance DecOptappears_free_in_tm__bindings_nonrec_sound bs tm : DecOptSoundPos (appears_free_in_tm__bindings_nonrec bs tm).
 Proof. derive__sound (appears_free_in_tm_proxy_sound (appears_free_in_tm__bindings_nonrec_tag bs tm)). Qed.
 
+Instance DecOptappears_free_in_tm__bindings_nonrec_complete bs tm : DecOptCompletePos (appears_free_in_tm__bindings_nonrec bs tm).
+Proof. derive__complete (appears_free_in_tm_proxy_complete). Qed.
+
+Instance DecOptappears_free_in_tm__bindings_nonrec_mon name tm: DecOptSizeMonotonic (appears_free_in_tm__bindings_nonrec name tm).
+Proof. apply DecOptappears_free_in_tm_proxy_mon. Qed.
+
 
 
 (* appears_free_in_tm__bindings_rec *)
@@ -73,6 +136,13 @@ Instance DecOptappears_free_in_tm__bindings_rec bs tm : DecOpt (appears_free_in_
 Instance DecOptappears_free_in_tm__bindings_rec_sound bs tm : DecOptSoundPos (appears_free_in_tm__bindings_rec bs tm).
 Proof. derive__sound (appears_free_in_tm_proxy_sound (appears_free_in_tm__bindings_rec_tag bs tm)). Qed.
 
+Instance DecOptappears_free_in_tm__bindings_rec_complete bs tm : DecOptCompletePos (appears_free_in_tm__bindings_rec bs tm).
+Proof. derive__complete (appears_free_in_tm_proxy_complete). Qed.
+
+Instance DecOptappears_free_in_tm__bindings_rec_mon name tm: DecOptSizeMonotonic (appears_free_in_tm__bindings_rec name tm).
+Proof. apply DecOptappears_free_in_tm_proxy_mon. Qed.
+
+
 
 (* appears_free_in_tm__binding *)
 
@@ -82,6 +152,11 @@ Instance DecOptappears_free_in_tm__binding bs tm : DecOpt (appears_free_in_tm__b
 Instance DecOptappears_free_in_tm__binding_sound bs tm : DecOptSoundPos (appears_free_in_tm__binding bs tm).
 Proof. derive__sound (appears_free_in_tm_proxy_sound (appears_free_in_tm__binding_tag bs tm)). Qed.
 
+Instance DecOptappears_free_in_tm__binding_complete bs tm : DecOptCompletePos (appears_free_in_tm__binding bs tm).
+Proof. derive__complete (appears_free_in_tm_proxy_complete). Qed.
+
+Instance DecOptappears_free_in_tm__binding_mon name tm: DecOptSizeMonotonic (appears_free_in_tm__binding name tm).
+Proof. apply DecOptappears_free_in_tm_proxy_mon. Qed.
 
 
 
